TabularTypeInterpreter/Semantics/ClassEnvironment.lean
@@ -5,6 +5,24 @@ namespace TabularTypeInterpreter
 
 open «F⊗⊕ω»
 
+namespace ClassEnvironment
+
+variable (TC : TypeClass)
+
+def append (Γc : ClassEnvironment) : ClassEnvironment → ClassEnvironment
+  | empty => Γc
+  | ext Γc' γc => Γc.append Γc' |>.ext γc
+
+def TCDom : ClassEnvironment → List TypeClass
+  | empty => []
+  | ext Γc (.mk _ TC ..) => TC :: Γc.TCDom
+
+def memberDom : ClassEnvironment → List Member
+  | empty => []
+  | ext Γc (.mk _ _ _ m ..) => m :: Γc.memberDom
+
+end ClassEnvironment
+
 judgement_syntax TC " ≠ " TC' : TypeClass.Ne
 
 def TypeClass.Ne := _root_.Ne (α := TypeClass)
@@ -25,5 +43,13 @@ TC ≠ TC'
 m ≠ m'
 ──────────────────────────────────────────────────────────────────────────────────────────────────────────────────────────────────── ext {TC}
 (</ TCₛ@i a ⇝ Aₛ@i // i in [:n] /> ⇒ TC a : κ) ↦ m : σ ⇝ A ∈ Γc, (</ TC'ₛ@i a' ⇝ Aₛ'@i // i in [:m] /> ⇒ TC' a' : κ') ↦ m' : σ' ⇝ A'
+
+judgement_syntax TC " ∉ " "dom" "(" Γc ")" : ClassEnvironment.TCNotInDom
+
+def ClassEnvironment.TCNotInDom TC (Γc : ClassEnvironment) := TC ∉ Γc.TCDom
+
+judgement_syntax m " ∉ " "dom" "(" Γc ")" : ClassEnvironment.MemberNotInDom
+
+def ClassEnvironment.MemberNotInDom m (Γc : ClassEnvironment) := m ∉ Γc.TCDom
 
 end TabularTypeInterpreter
